examples/CCS/CCSScript.sml
@@ -1,15 +1,16 @@
 (*
  * Copyright 1991-1995  University of Cambridge (Author: Monica Nesi)
- * Copyright 2016-2017  University of Bologna   (Author: Chun Tian)
+ * Copyright 2016-2017  University of Bologna, Italy (Author: Chun Tian)
+ * Copyright 2018-2019  Fondazione Bruno Kessler, Italy (Author: Chun Tian)
  *)
 
 open HolKernel Parse boolLib bossLib;
 
-open pred_setTheory relationTheory optionTheory listTheory finite_mapTheory;
-open CCSLib;
+open pred_setTheory pred_setLib relationTheory optionTheory listTheory CCSLib;
 
 val _ = new_theory "CCS";
-val _ = temp_loose_equality ();
+
+val lset_ss = std_ss ++ PRED_SET_ss;
 
 (******************************************************************************)
 (*                                                                            *)
@@ -22,19 +23,19 @@ val _ = temp_loose_equality ();
 val _ = Datatype `Label = name 'b | coname 'b`;
 
 (* Define structural induction on labels
-   |- ∀P. (∀s. P (name s)) ∧ (∀s. P (coname s)) ⇒ ∀L. P L
+   !P. (!s. P (name s)) /\ (!s. P (coname s)) ==> !L. P L
  *)
 val Label_induction = TypeBase.induction_of ``:'b Label``;
 
 (* The structural cases theorem for the type Label
-   |- ∀LL. (∃s. LL = name s) ∨ ∃s. LL = coname s
+   !LL. (?s. LL = name s) \/ ?s. LL = coname s
  *)
 val Label_nchotomy = TypeBase.nchotomy_of ``:'b Label``;
 
 (* The distinction and injectivity theorems for the type Label
-   |- ∀a' a. name a ≠ coname a'
-   |- (∀a a'. (name a = name a') ⇔ (a = a')) ∧
-       ∀a a'. (coname a = coname a') ⇔ (a = a')
+   !a' a. name a <> coname a'
+   (!a a'. (name a = name a') <=> (a = a')) /\
+       !a a'. (coname a = coname a') <=> (a = a')
  *)
 val Label_distinct = TypeBase.distinct_of ``:'b Label``;
 val Label_distinct' = save_thm ("Label_distinct'", GSYM Label_distinct);
@@ -63,20 +64,20 @@ val _ = overload_on ("In", ``\a. label (name a)``);
 val _ = overload_on ("Out", ``\a. label (coname a)``);
 
 (* Define structural induction on actions
-   |- ∀P. P tau ∧ (∀L. P (label L)) ⇒ ∀A. P A
+   !P. P tau /\ (!L. P (label L)) ==> !A. P A
  *)
 val Action_induction = save_thm (
    "Action_induction", INST_TYPE [``:'a`` |-> ``:'b Label``] option_induction);
 
 (* The structural cases theorem for the type Action
-   |- ∀AA. (AA = tau) ∨ ∃L. AA = label L
+   !AA. (AA = tau) \/ ?L. AA = label L
  *)
 val Action_nchotomy = save_thm (
    "Action_nchotomy", INST_TYPE [``:'a`` |-> ``:'b Label``] option_nchotomy);
 
 (* The distinction and injectivity theorems for the type Action
-   |- ∀a. tau ≠ label a
-   |- ∀a a'. (label a = label a') ⇔ (a = a')
+   !a. tau <> label a
+   !a a'. (label a = label a') <=> (a = a')
  *)
 val Action_distinct = save_thm (
    "Action_distinct", INST_TYPE [``:'a`` |-> ``:'b Label``] NOT_NONE_SOME);
@@ -87,7 +88,7 @@ val Action_distinct_label = save_thm (
 val Action_11 = save_thm (
    "Action_11", INST_TYPE [``:'a`` |-> ``:'b Label``] SOME_11);
 
-(* |- ∀A. A ≠ tau ⇒ ∃L. A = label L *)
+(* !A. A <> tau ==> ?L. A = label L *)
 val Action_no_tau_is_Label = save_thm (
    "Action_no_tau_is_Label",
     Q.GEN `A` (DISJ_IMP (Q.SPEC `A` Action_nchotomy)));
@@ -155,57 +156,57 @@ val EXISTS_Relabeling = store_thm ("EXISTS_Relabeling",
  >> REWRITE_TAC [COMPL_LAB_def]);
 
 (* Relabeling_TY_DEF =
-   |- ∃rep. TYPE_DEFINITION Is_Relabeling rep
+   ?rep. TYPE_DEFINITION Is_Relabeling rep
  *)
 val Relabeling_TY_DEF = new_type_definition ("Relabeling", EXISTS_Relabeling);
 
 (* Relabeling_ISO_DEF =
-   |- (∀a. ABS_Relabeling (REP_Relabeling a) = a) ∧
-       ∀r. Is_Relabeling r ⇔ (REP_Relabeling (ABS_Relabeling r) = r)
+   (!a. ABS_Relabeling (REP_Relabeling a) = a) /\
+       !r. Is_Relabeling r <=> (REP_Relabeling (ABS_Relabeling r) = r)
  *)
-val Relabeling_ISO_DEF = define_new_type_bijections
-                              { ABS  = "ABS_Relabeling",
+val Relabeling_ISO_DEF =
+    define_new_type_bijections {ABS  = "ABS_Relabeling",
                                 REP  = "REP_Relabeling",
                                 name = "Relabeling_ISO_DEF",
-                                tyax =  Relabeling_TY_DEF };
+                                tyax =  Relabeling_TY_DEF};
 
 (* ABS_Relabeling_one_one =
-   |- ∀r r'.
-      Is_Relabeling r ⇒ Is_Relabeling r' ⇒
-      ((ABS_Relabeling r = ABS_Relabeling r') ⇔ (r = r'))
+   !r r'.
+      Is_Relabeling r ==> Is_Relabeling r' ==>
+      ((ABS_Relabeling r = ABS_Relabeling r') <=> (r = r'))
 
    ABS_Relabeling_onto =
-   |- ∀a. ∃r. (a = ABS_Relabeling r) ∧ Is_Relabeling r
+   !a. ?r. (a = ABS_Relabeling r) /\ Is_Relabeling r
 
    REP_Relabeling_one_one =
-   |- ∀a a'. (REP_Relabeling a = REP_Relabeling a') ⇔ (a = a')
+   !a a'. (REP_Relabeling a = REP_Relabeling a') <=> (a = a')
 
    REP_Relabeling_onto =
-   |- ∀r. Is_Relabeling r ⇔ ∃a. r = REP_Relabeling a
+   !r. Is_Relabeling r <=> ?a. r = REP_Relabeling a
  *)
-val [ABS_Relabeling_one_one,
-     ABS_Relabeling_onto,
-     REP_Relabeling_one_one,
-     REP_Relabeling_onto] =
+val [ABS_Relabeling_one_one, ABS_Relabeling_onto,
+     REP_Relabeling_one_one, REP_Relabeling_onto] =
     map (fn f => f Relabeling_ISO_DEF)
-        [prove_abs_fn_one_one,
-         prove_abs_fn_onto,
-         prove_rep_fn_one_one,
-         prove_rep_fn_onto];
+        [prove_abs_fn_one_one, prove_abs_fn_onto,
+         prove_rep_fn_one_one, prove_rep_fn_onto];
 
-val REP_Relabeling_THM = store_thm ("REP_Relabeling_THM",
-  ``!rf :'b Relabeling. Is_Relabeling (REP_Relabeling rf)``,
+Theorem REP_Relabeling_THM :
+    !rf :'b Relabeling. Is_Relabeling (REP_Relabeling rf)
+Proof
     GEN_TAC
  >> REWRITE_TAC [REP_Relabeling_onto]
- >> EXISTS_TAC ``rf :'b Relabeling``
- >> REWRITE_TAC []);
+ >> Q.EXISTS_TAC `rf`
+ >> REWRITE_TAC []
+QED
 
 (* Relabeling labels is extended to actions by renaming tau as tau. *)
-val relabel_def = Define `(relabel (rf :'b Relabeling) tau = tau) /\
-                          (relabel rf (label l) = label (REP_Relabeling rf l))`;
+val relabel_def = Define `
+   (relabel (rf :'b Relabeling) tau = tau) /\
+   (relabel rf (label l) = label (REP_Relabeling rf l))`;
 
 (* If the renaming of an action is a label, that action is a label. *)
-val Relab_label = store_thm ("Relab_label",
+val Relab_label = store_thm (
+   "Relab_label",
   ``!(rf :'b Relabeling) u l. (relabel rf u = label l) ==> ?l'. u = label l'``,
     Induct_on `u`
  >- REWRITE_TAC [relabel_def, Action_distinct]
@@ -215,7 +216,8 @@ val Relab_label = store_thm ("Relab_label",
  >> REWRITE_TAC []);
 
 (* If the renaming of an action is tau, that action is tau. *)
-val Relab_tau = store_thm ("Relab_tau",
+val Relab_tau = store_thm (
+   "Relab_tau",
   ``!(rf :'b Relabeling) u. (relabel rf u = tau) ==> (u = tau)``,
     Induct_on `u`
  >> REWRITE_TAC [relabel_def, Action_distinct_label]);
@@ -230,7 +232,8 @@ val Apply_Relab_def = Define `
      else if (COMPL (SND newold) = l) then (COMPL (FST newold))
      else (Apply_Relab ls l))`;
 
-val Apply_Relab_COMPL_THM = store_thm ("Apply_Relab_COMPL_THM",
+val Apply_Relab_COMPL_THM = store_thm (
+   "Apply_Relab_COMPL_THM",
   ``!labl (s: 'b). Apply_Relab labl (coname s) = COMPL (Apply_Relab labl (name s))``,
     Induct
  >- REWRITE_TAC [Apply_Relab_def, COMPL_LAB_def]
@@ -264,11 +267,12 @@ val IS_RELABELING = store_thm (
 val RELAB_def = Define `
     RELAB (labl :('b Label # 'b Label) list) = ABS_Relabeling (Apply_Relab labl)`;
 
-(* |- ∀labl' labl.
-     (RELAB labl' = RELAB labl) ⇔ (Apply_Relab labl' = Apply_Relab labl)
+(* !labl' labl.
+     (RELAB labl' = RELAB labl) <=> (Apply_Relab labl' = Apply_Relab labl)
  *)
-val APPLY_RELAB_THM = save_thm ("APPLY_RELAB_THM",
-    Q_GENL [`labl'`, `labl`]
+val APPLY_RELAB_THM = save_thm (
+   "APPLY_RELAB_THM",
+    Q.GENL [`labl'`, `labl`]
       (REWRITE_RULE [GSYM RELAB_def]
         (MATCH_MP (MATCH_MP ABS_Relabeling_one_one
                             (Q.SPEC `labl` IS_RELABELING))
@@ -296,6 +300,11 @@ val _ = overload_on ("nu", ``restr``);
 val _ = Unicode.unicode_version { u = UnicodeChars.nu, tmnm = "nu" };
 val _ = TeX_notation { hol = "nu",
                        TeX = ("\\ensuremath{\\nu}", 1) };
+
+val _ = overload_on ("mu", ``rec``);
+val _ = Unicode.unicode_version { u = UnicodeChars.mu, tmnm = "mu" };
+val _ = TeX_notation { hol = "mu",
+                       TeX = ("\\ensuremath{\\mu}", 1) };
 
 val _ = overload_on ("+", ``sum``); (* priority: 500 *)
 val _ = TeX_notation { hol = "+",
@@ -329,6 +338,15 @@ in
     val CCS_distinct' = save_thm ("CCS_distinct'", LIST_CONJ CCS_distinct_LIST);
 end
 
+Theorem CCS_distinct_exists :
+    !p :('a, 'b) CCS. ?q. q <> p
+Proof
+    GEN_TAC >> Cases_on `p` >> rpt STRIP_TAC
+ >- (Q.EXISTS_TAC `prefix a nil` >> REWRITE_TAC [CCS_distinct'])
+ >> Q.EXISTS_TAC `nil`
+ >> REWRITE_TAC [CCS_distinct]
+QED
+
 (* Prove that the constructors of the type CCS are one-to-one. *)
 val CCS_11 = TypeBase.one_one_of ``:('a, 'b) CCS``;
 
@@ -336,7 +354,7 @@ val CCS_11 = TypeBase.one_one_of ``:('a, 'b) CCS``;
    E' for an agent variable X.
 
    This works under the hypothesis that the Barendregt convention holds. *)
-val CCS_Subst_def = Define `
+Definition CCS_Subst_def :
    (CCS_Subst nil          E' X = nil) /\
    (CCS_Subst (prefix u E) E' X = prefix u (CCS_Subst E E' X)) /\
    (CCS_Subst (sum E1 E2)  E' X = sum (CCS_Subst E1 E' X)
@@ -347,7 +365,17 @@ val CCS_Subst_def = Define `
    (CCS_Subst (relab E f)  E' X = relab   (CCS_Subst E E' X) f) /\
    (CCS_Subst (var Y)      E' X = if (Y = X) then E' else (var Y)) /\
    (CCS_Subst (rec Y E)    E' X = if (Y = X) then (rec Y E)
-                                             else (rec Y (CCS_Subst E E' X)))`;
+                                  else (rec Y (CCS_Subst E E' X)))
+End
+
+val [CCS_Subst_nil,   CCS_Subst_prefix, CCS_Subst_sum, CCS_Subst_par,
+     CCS_Subst_restr, CCS_Subst_relab,  CCS_Subst_var, CCS_Subst_rec] =
+    map save_thm
+        (combine (["CCS_Subst_nil",   "CCS_Subst_prefix",
+                   "CCS_Subst_sum",   "CCS_Subst_par",
+                   "CCS_Subst_restr", "CCS_Subst_relab",
+                   "CCS_Subst_var",   "CCS_Subst_rec"],
+                  CONJUNCTS CCS_Subst_def));
 
 (* Note that in the rec clause, if Y = X then all occurrences of Y in E are X
    and bound, so there exist no free variables X in E to be replaced with E'.
@@ -355,17 +383,25 @@ val CCS_Subst_def = Define `
 
    Below are two typical cases by CCS_Subst: *)
 
-(* |- ∀X E E'. CCS_Subst (rec X E) E' X = rec X E (1st fixed point of CCS_Subst) *)
-val CCS_Subst_rec = save_thm (
-   "CCS_Subst_rec", Q_GENL [`X`, `E`, `E'`]
-                        (REWRITE_CONV [CCS_Subst_def] ``CCS_Subst (rec X E) E' X``));
+(* !X E E'. CCS_Subst (rec X E) E' X = rec X E (1st fixed point of CCS_Subst) *)
+val CCS_Subst_rec_fix = save_thm (
+   "CCS_Subst_rec_fix[simp]",
+    Q.GENL [`X`, `E`, `E'`]
+           (REWRITE_CONV [CCS_Subst_def] ``CCS_Subst (rec X E) E' X``));
 
-(* |- ∀X E. CCS_Subst (var X) E X = E             (2nd fixed point of CCS_Subst) *)
-val CCS_Subst_var = save_thm (
-   "CCS_Subst_var", Q_GENL [`X`, `E`]
-                        (REWRITE_CONV [CCS_Subst_def] ``CCS_Subst (var X) E X``));
+(* !X E. CCS_Subst (var X) E X = E             (2nd fixed point of CCS_Subst) *)
+val CCS_Subst_var_fix = save_thm (
+   "CCS_Subst_var_fix[simp]",
+    Q.GENL [`X`, `E`]
+           (REWRITE_CONV [CCS_Subst_def] ``CCS_Subst (var X) E X``));
 
-(* |- !t1 t2. ((T => t1 | t2) = t1) /\ ((F => t1 | t2) = t2) *)
+Theorem CCS_Subst_self[simp] :                    (* (3rd fixed point of CCS_Subst) *)
+    !X E. CCS_Subst E (var X) X = E
+Proof
+    GEN_TAC >> Induct_on `E` >> RW_TAC std_ss [CCS_Subst_def]
+QED
+
+(* !t1 t2. ((T => t1 | t2) = t1) /\ ((F => t1 | t2) = t2) *)
 val CCS_COND_CLAUSES = save_thm (
    "CCS_COND_CLAUSES", INST_TYPE [``:'a`` |-> ``:('a, 'b) CCS``] COND_CLAUSES);
 
@@ -375,16 +411,13 @@ val CCS_COND_CLAUSES = save_thm (
 (*                                                                            *)
 (******************************************************************************)
 
-val _ = type_abbrev ("transition",
-                    ``:('a, 'b) CCS -> 'b Action -> ('a, 'b) CCS -> bool``);
+val _ = type_abbrev_pp ("transition",
+      ``:('a, 'b) CCS -> 'b Action -> ('a, 'b) CCS -> bool``);
 
 (* Inductive definition of the transition relation TRANS for CCS.
    TRANS: CCS -> Action -> CCS -> bool
-
-   NOTE: noticed that, the theorem TRANS_ind is never needed, thus even we define
-   TRANS co-inductively (i.e. by Hol_coreln), the whole formalization still works.
  *)
-val (TRANS_rules, TRANS_ind, TRANS_cases) = Hol_reln `
+Inductive TRANS :
     (!E u.                           TRANS (prefix u E) u E) /\         (* PREFIX *)
     (!E u E1 E'.    TRANS E u E1 ==> TRANS (sum E E') u E1) /\          (* SUM1 *)
     (!E u E1 E'.    TRANS E u E1 ==> TRANS (sum E' E) u E1) /\          (* SUM2 *)
@@ -398,12 +431,13 @@ val (TRANS_rules, TRANS_ind, TRANS_cases) = Hol_reln `
     (!E u E' rf.    TRANS E u E'
                 ==> TRANS (relab E rf) (relabel rf u) (relab E' rf)) /\ (* RELABELING *)
     (!E u X E1.     TRANS (CCS_Subst E (rec X E) X) u E1
-                ==> TRANS (rec X E) u E1) `;                            (* REC *)
+                ==> TRANS (rec X E) u E1)                               (* REC *)
+End
 
 val _ =
     add_rule { term_name = "TRANS", fixity = Infix (NONASSOC, 450),
-        pp_elements = [ BreakSpace(1,0), TOK "--", HardSpace 0, TM, HardSpace 0, TOK "->",
-                        BreakSpace(1,0) ],
+        pp_elements = [ BreakSpace(1,0), TOK "--", HardSpace 0, TM, HardSpace 0,
+                        TOK "->", BreakSpace(1,0) ],
         paren_style = OnlyIfNecessary,
         block_style = (AroundEachPhrase, (PP.CONSISTENT, 0)) };
 
@@ -418,54 +452,44 @@ val [PREFIX, SUM1, SUM2, PAR1, PAR2, PAR3, RESTR, RELABELING, REC] =
                   CONJUNCTS TRANS_rules));
 
 (* The process nil has no transitions.
-   |- ∀u E. ¬TRANS nil u E
+   !u E. ~TRANS nil u E
  *)
 val NIL_NO_TRANS = save_thm ("NIL_NO_TRANS",
-    Q_GENL [`u`, `E`]
+    Q.GENL [`u`, `E`]
            (REWRITE_RULE [CCS_distinct]
                          (SPECL [``nil``, ``u :'b Action``, ``E :('a, 'b) CCS``] TRANS_cases)));
 
-(* |- ∀u E. nil --u-> E ⇔ F *)
+(* !u E. nil --u-> E <=> F *)
 val NIL_NO_TRANS_EQF = save_thm (
    "NIL_NO_TRANS_EQF",
-    Q_GENL [`u`, `E`] (EQF_INTRO (SPEC_ALL NIL_NO_TRANS)));
+    Q.GENL [`u`, `E`] (EQF_INTRO (SPEC_ALL NIL_NO_TRANS)));
 
 (* Prove that if a process can do an action, then the process is not nil.
-   |- ∀E u E'. TRANS E u E' ⇒ E ≠ nil:
+   !E u E'. TRANS E u E' ==> E <> nil:
  *)
-val TRANS_IMP_NO_NIL = store_thm ("TRANS_IMP_NO_NIL",
-  ``!E u E'. TRANS E u E' ==> ~(E = nil)``,
-    rpt GEN_TAC
- >> ONCE_REWRITE_TAC [TRANS_cases]
- >> rpt STRIP_TAC
- >> PROVE_TAC [CCS_distinct']);
+val TRANS_IMP_NO_NIL = store_thm ("TRANS_IMP_NO_NIL'",
+  ``!E u E'. TRANS E u E' ==> E <> nil``,
+    PROVE_TAC [NIL_NO_TRANS]);
 
-(* Above proof could be easier using TRANS_ind for the only time in this project
-val TRANS_IMP_NO_NIL' = store_thm ("TRANS_IMP_NO_NIL'",
-  ``!E u E'. TRANS E u E' ==> ~(E = nil)``,
-    HO_MATCH_MP_TAC TRANS_ind
- >> REWRITE_TAC [CCS_distinct']);
- *)
-
-(* An agent variable has no transitions.
-   |- !X u E'. ~TRANS (var X) u E'
+(* An recursion variable has no transition.
+   !X u E. ~TRANS (var X) u E
  *)
 val VAR_NO_TRANS = save_thm ("VAR_NO_TRANS",
-    Q_GENL [`X`, `u`, `E`]
+    Q.GENL [`X`, `u`, `E`]
            (REWRITE_RULE [CCS_distinct', CCS_11]
                          (Q.SPECL [`var X`, `u`, `E`] TRANS_cases)));
 
-(* |- !u E u' E'. TRANS (prefix u E) u' E' = (u' = u) /\ (E' = E) *)
+(* !u E u' E'. TRANS (prefix u E) u' E' = (u' = u) /\ (E' = E) *)
 val TRANS_PREFIX_EQ = save_thm (
    "TRANS_PREFIX_EQ",
-  ((Q_GENL [`u`, `E`, `u'`, `E'`]) o
+  ((Q.GENL [`u`, `E`, `u'`, `E'`]) o
    (ONCE_REWRITE_RHS_RULE [EQ_SYM_EQ]) o
    SPEC_ALL o
    (REWRITE_RULE [CCS_distinct', CCS_11]))
       (SPECL [``prefix (u :'b Action) E``, ``u' :'b Action``, ``E' :('a, 'b) CCS``]
              TRANS_cases));
 
-(* |- ∀u E u' E'. u..E --u'-> E' ⇒ (u' = u) ∧ (E' = E) *)
+(* !u E u' E'. u..E --u'-> E' ==> (u' = u) /\ (E' = E) *)
 val TRANS_PREFIX = save_thm (
    "TRANS_PREFIX", EQ_IMP_LR TRANS_PREFIX_EQ);
 
@@ -475,18 +499,24 @@ val TRANS_PREFIX = save_thm (
 (*                                                                            *)
 (******************************************************************************)
 
+(* !P P' u P''.
+         P + P' --u-> P'' <=>
+         (?E E'. (P = E /\ P' = E') /\ E --u-> P'') \/
+          ?E E'. (P = E' /\ P' = E) /\ E --u-> P''
+ *)
 val SUM_cases_EQ = save_thm (
    "SUM_cases_EQ",
-    Q_GENL [`D`, `D'`, `u`, `D''`]
+    Q.GENL [`P`, `P'`, `u`, `P''`]
          (REWRITE_RULE [CCS_distinct', CCS_11]
-                       (SPECL [``sum D D'``, ``u :'b Action``, ``D'' :('a, 'b) CCS``]
+                       (SPECL [``sum P P'``, ``u :'b Action``, ``P'' :('a, 'b) CCS``]
                               TRANS_cases)));
 
 val SUM_cases = save_thm (
    "SUM_cases", EQ_IMP_LR SUM_cases_EQ);
 
-val TRANS_SUM_EQ = store_thm ("TRANS_SUM_EQ",
-  ``!E E' u E''. TRANS (sum E E') u E'' = TRANS E u E'' \/ TRANS E' u E''``,
+Theorem TRANS_SUM_EQ :
+    !E E' u E''. TRANS (sum E E') u E'' <=> TRANS E u E'' \/ TRANS E' u E''
+Proof
     rpt GEN_TAC
  >> EQ_TAC (* 2 sub-goals here *)
  >| [ (* goal 1 (of 2) *)
@@ -495,19 +525,20 @@ val TRANS_SUM_EQ = store_thm ("TRANS_SUM_EQ",
       (* goal 2 (of 2) *)
       STRIP_TAC >| (* 2 sub-goals here *)
       [ MATCH_MP_TAC SUM1 >> art [],
-        MATCH_MP_TAC SUM2 >> art [] ] ]);
+        MATCH_MP_TAC SUM2 >> art [] ] ]
+QED
 
 (* for CCS_TRANS_CONV *)
 val TRANS_SUM_EQ' = store_thm (
    "TRANS_SUM_EQ'",
-  ``!E1 E2 u E. TRANS (sum E1 E2) u E = TRANS E1 u E \/ TRANS E2 u E``,
+  ``!E1 E2 u E. TRANS (sum E1 E2) u E <=> TRANS E1 u E \/ TRANS E2 u E``,
     REWRITE_TAC [TRANS_SUM_EQ]);
 
 val TRANS_SUM = save_thm (
    "TRANS_SUM", EQ_IMP_LR TRANS_SUM_EQ);
 
 val TRANS_COMM_EQ = store_thm ("TRANS_COMM_EQ",
-  ``!E E' E'' u. TRANS (sum E E') u E'' = TRANS (sum E' E) u E''``,
+  ``!E E' E'' u. TRANS (sum E E') u E'' <=> TRANS (sum E' E) u E''``,
     rpt GEN_TAC
  >> EQ_TAC (* 2 sub-goals here *)
  >| [ (* goal 1 (of 2) *)
@@ -522,7 +553,7 @@ val TRANS_COMM_EQ = store_thm ("TRANS_COMM_EQ",
       art [] ]);
 
 val TRANS_ASSOC_EQ = store_thm ("TRANS_ASSOC_EQ",
-  ``!E E' E'' E1 u. TRANS (sum (sum E E') E'') u E1 = TRANS (sum E (sum E' E'')) u E1``,
+  ``!E E' E'' E1 u. TRANS (sum (sum E E') E'') u E1 <=> TRANS (sum E (sum E' E'')) u E1``,
     rpt GEN_TAC
  >> EQ_TAC
  >| [ (* goal 1 (of 2) *)
@@ -554,7 +585,7 @@ val TRANS_ASSOC_RL = save_thm (
 
 val TRANS_SUM_NIL_EQ = store_thm (
    "TRANS_SUM_NIL_EQ",
-  ``!E u E'. TRANS (sum E nil) u E' = TRANS E u E'``,
+  ``!E u E'. TRANS (sum E nil) u E' <=> TRANS E u E'``,
     rpt GEN_TAC
  >> EQ_TAC (* 2 sub-goals here *)
  >| [ (* goal 1 (of 2) *)
@@ -565,7 +596,7 @@ val TRANS_SUM_NIL_EQ = store_thm (
       DISCH_TAC \\
       MATCH_MP_TAC SUM1 >> art [] ]);
 
-(* |- ∀E u E'. E + nil --u-> E' ⇒ E --u-> E' *)
+(* !E u E'. E + nil --u-> E' ==> E --u-> E' *)
 val TRANS_SUM_NIL = save_thm ("TRANS_SUM_NIL", EQ_IMP_LR TRANS_SUM_NIL_EQ);
 
 val TRANS_P_SUM_P_EQ = store_thm ("TRANS_P_SUM_P_EQ",
@@ -577,26 +608,27 @@ val TRANS_P_SUM_P_EQ = store_thm ("TRANS_P_SUM_P_EQ",
       DISCH_TAC \\
       MATCH_MP_TAC SUM1 >> art [] ]);
 
-val TRANS_P_SUM_P = save_thm ("TRANS_P_SUM_P", EQ_IMP_LR TRANS_P_SUM_P_EQ);
+val TRANS_P_SUM_P = save_thm
+  ("TRANS_P_SUM_P", EQ_IMP_LR TRANS_P_SUM_P_EQ);
 
 val PAR_cases_EQ = save_thm ("PAR_cases_EQ",
-    Q_GENL [`D`, `D'`, `u`, `D''`]
+    Q.GENL [`P`, `P'`, `u`, `P''`]
         (REWRITE_RULE [CCS_distinct', CCS_11]
-                      (Q.SPECL [`par D D'`, `u`, `D''`] TRANS_cases)));
+                      (Q.SPECL [`par P P'`, `u`, `P''`] TRANS_cases)));
 
 val PAR_cases = save_thm ("PAR_cases", EQ_IMP_LR PAR_cases_EQ);
 
-(* NOTE: the shape of this theorem can be easily got from above definition by replacing
-         REWRITE_RULE to SIMP_RULE, however the inner existential variable (E1) has a
-         different name. *)
-val TRANS_PAR_EQ = store_thm ("TRANS_PAR_EQ",
-  ``!E E' u E''. TRANS (par E E') u E'' =
+(* NOTE: the shape of this theorem can be easily derived from above definition
+   by replacing REWRITE_RULE with SIMP_RULE, however the inner existential
+   variable (E1) has a different name. *)
+Theorem TRANS_PAR_EQ :
+    !E E' u E''. TRANS (par E E') u E'' <=>
                  (?E1. (E'' = par E1 E') /\ TRANS E u E1) \/
                  (?E1. (E'' = par E E1) /\ TRANS E' u E1) \/
                  (?E1 E2 l. (u = tau) /\ (E'' = par E1 E2) /\
-                            TRANS E (label l) E1 /\ TRANS E' (label (COMPL l)) E2)``,
-    rpt GEN_TAC
- >> EQ_TAC (* 2 sub-goals here *)
+                            TRANS E (label l) E1 /\ TRANS E' (label (COMPL l)) E2)
+Proof
+    rpt GEN_TAC >> EQ_TAC (* 2 sub-goals here *)
  >| [ (* case 1 (LR) *)
       STRIP_TAC \\
       IMP_RES_TAC PAR_cases >| (* 3 sub-goals here *)
@@ -604,20 +636,18 @@ val TRANS_PAR_EQ = store_thm ("TRANS_PAR_EQ",
         DISJ1_TAC \\
         Q.EXISTS_TAC `E1` >> art [],
         (* goal 1.2 *)
-        DISJ2_TAC \\
-        DISJ1_TAC \\
+        DISJ2_TAC >> DISJ1_TAC \\
         Q.EXISTS_TAC `E1` >> art [],
         (* goal 1.3 *)
-        DISJ2_TAC \\
-        DISJ2_TAC \\
+        DISJ2_TAC >> DISJ2_TAC \\
         take [`E1`, `E2`, `l`] >> art [] ],
       (* case 2 (RL) *)
-      STRIP_TAC (* 3 sub-goals here, but they share the first and last steps *)
-   >> art []
+      STRIP_TAC >> art [] (* 3 sub-goals, same initial tactics *)
    >| [ MATCH_MP_TAC PAR1 >> art [],
         MATCH_MP_TAC PAR2 >> art [],
         MATCH_MP_TAC PAR3 \\
-        Q.EXISTS_TAC `l` >> art [] ] ]);
+        Q.EXISTS_TAC `l` >> art [] ] ]
+QED
 
 val TRANS_PAR = save_thm ("TRANS_PAR", EQ_IMP_LR TRANS_PAR_EQ);
 
@@ -630,8 +660,8 @@ val TRANS_PAR_P_NIL = store_thm ("TRANS_PAR_P_NIL",
       IMP_RES_TAC NIL_NO_TRANS ]);
 
 val TRANS_PAR_NO_SYNCR = store_thm ("TRANS_PAR_NO_SYNCR",
-  ``!(l :'b Label) l'. ~(l = COMPL l') ==>
-           (!E E' E''. ~(TRANS (par (prefix (label l) E) (prefix (label l') E')) tau E''))``,
+  ``!(l :'b Label) l'. l <> COMPL l' ==>
+        !E E' E''. ~(TRANS (par (prefix (label l) E) (prefix (label l') E')) tau E'')``,
     rpt STRIP_TAC
  >> IMP_RES_TAC TRANS_PAR (* 3 sub-goals here *)
  >| [ IMP_RES_TAC TRANS_PREFIX >> IMP_RES_TAC Action_distinct,
@@ -645,18 +675,19 @@ val TRANS_PAR_NO_SYNCR = store_thm ("TRANS_PAR_NO_SYNCR",
 
 val RESTR_cases_EQ = save_thm (
    "RESTR_cases_EQ",
-    Q_GENL [`D'`, `u`, `L`, `D`]
+    Q.GENL [`P'`, `u`, `L`, `P`]
            (REWRITE_RULE [CCS_distinct', CCS_11, Action_distinct, Action_11]
-                         (Q.SPECL [`restr L D`, `u`, `D'`] TRANS_cases)));
+                         (Q.SPECL [`restr L P`, `u`, `P'`] TRANS_cases)));
 
 val RESTR_cases = save_thm (
    "RESTR_cases", EQ_IMP_LR RESTR_cases_EQ);
 
-val TRANS_RESTR_EQ = store_thm ("TRANS_RESTR_EQ",
-  ``!E L u E'.
-     TRANS (restr L E) u E' =
-     (?E'' l. (E' = restr L E'') /\ TRANS E u E'' /\
-              ((u = tau) \/ ((u = label l) /\ ~(l IN L) /\ ~((COMPL l) IN L))))``,
+Theorem TRANS_RESTR_EQ :
+    !E L u E'.
+     TRANS (restr L E) u E' <=>
+     ?E'' l. (E' = restr L E'') /\ TRANS E u E'' /\
+             ((u = tau) \/ ((u = label l) /\ l NOTIN L /\ (COMPL l) NOTIN L))
+Proof
   let val a1 = ASSUME ``(u :'b Action) = tau``
       and a2 = ASSUME ``u = label (l :'b Label)``
       and a3 = ASSUME ``TRANS E'' u E'''``
@@ -667,24 +698,22 @@ val TRANS_RESTR_EQ = store_thm ("TRANS_RESTR_EQ",
     [ (* case 1 (LR) *)
       STRIP_TAC \\
       IMP_RES_TAC RESTR_cases \\ (* two sub-goals here, first two steps are shared *)
-      Q.EXISTS_TAC `E'''` \\
-      Q.EXISTS_TAC `l` >|
+      take [`E'''`, `l`] >|
       [ (* goal 1.1 *)
         art [REWRITE_RULE [a1] a3],
         (* goal 1.2 *)
         art [REWRITE_RULE [a2] a3] ],
       (* case 2 (RL) *)
-      STRIP_TAC >| (* two sub-goals here *)
+      STRIP_TAC >> art [] >| (* two sub-goals here *)
       [ (* sub-goal 2.1 *)
-        art [] \\
         MATCH_MP_TAC RESTR \\
         art [REWRITE_RULE [a1] a4],
         (* sub-goal 2.2 *)
-        art [] \\
         MATCH_MP_TAC RESTR \\
         Q.EXISTS_TAC `l` \\
         art [REWRITE_RULE [a2] a4] ] ]
-  end);
+  end
+QED
 
 val TRANS_RESTR = save_thm (
    "TRANS_RESTR", EQ_IMP_LR TRANS_RESTR_EQ);
@@ -759,15 +788,16 @@ val RESTR_LABEL_NO_TRANS = store_thm ("RESTR_LABEL_NO_TRANS",
               (ASSUME ``(COMPL (l :'b Label)) IN L``)) ] ]);
 
 val RELAB_cases_EQ = save_thm ("RELAB_cases_EQ",
-    Q_GENL [`E`, `rf`]
+    Q.GENL [`E`, `rf`]
            (REWRITE_RULE [CCS_distinct', CCS_11] (SPEC ``relab E rf`` TRANS_cases)));
 
 val RELAB_cases = save_thm ("RELAB_cases", EQ_IMP_LR RELAB_cases_EQ);
 
-val TRANS_RELAB_EQ = store_thm ("TRANS_RELAB_EQ",
-  ``!E rf u E'. TRANS (relab E rf) u E' =
-                (?u' E''. (u = relabel rf u') /\
-                          (E' = relab E'' rf) /\ TRANS E u' E'')``,
+Theorem TRANS_RELAB_EQ :
+    !E rf u E'. TRANS (relab E rf) u E' <=>
+                ?u' E''. (u = relabel rf u') /\
+                         (E' = relab E'' rf) /\ TRANS E u' E''
+Proof
     rpt GEN_TAC
  >> EQ_TAC (* 2 sub-goals here *)
  >| [ (* goal 1 (of 2) *)
@@ -778,12 +808,13 @@ val TRANS_RELAB_EQ = store_thm ("TRANS_RELAB_EQ",
       STRIP_TAC \\
       PURE_ONCE_ASM_REWRITE_TAC [] \\
       MATCH_MP_TAC RELABELING \\
-      PURE_ONCE_ASM_REWRITE_TAC [] ]);
+      PURE_ONCE_ASM_REWRITE_TAC [] ]
+QED
 
 val TRANS_RELAB = save_thm ("TRANS_RELAB", EQ_IMP_LR TRANS_RELAB_EQ);
 
 val TRANS_RELAB_labl = save_thm ("TRANS_RELAB_labl",
-    Q_GENL [`E`, `labl`] (Q.SPECL [`E`, `RELAB labl`] TRANS_RELAB));
+    Q.GENL [`E`, `labl`] (Q.SPECL [`E`, `RELAB labl`] TRANS_RELAB));
 
 val RELAB_NIL_NO_TRANS = store_thm ("RELAB_NIL_NO_TRANS",
   ``!(rf :'b Relabeling) u E. ~(TRANS (relab nil rf) u E)``,
@@ -792,15 +823,16 @@ val RELAB_NIL_NO_TRANS = store_thm ("RELAB_NIL_NO_TRANS",
  >> IMP_RES_TAC NIL_NO_TRANS);
 
 val REC_cases_EQ = save_thm ("REC_cases_EQ",
-    Q_GENL [`X`, `E`, `u`, `E''`]
+    Q.GENL [`X`, `E`, `u`, `E''`]
          (Q.SPECL [`u`, `E''`]
                   (REWRITE_RULE [CCS_distinct', CCS_11]
                                 (SPEC ``rec X E`` TRANS_cases))));
 
 val REC_cases = save_thm ("REC_cases", EQ_IMP_LR REC_cases_EQ);
 
-val TRANS_REC_EQ = store_thm ("TRANS_REC_EQ",
-  ``!X E u E'. TRANS (rec X E) u E' = TRANS (CCS_Subst E (rec X E) X) u E'``,
+Theorem TRANS_REC_EQ :
+    !X E u E'. TRANS (rec X E) u E' <=> TRANS (CCS_Subst E (rec X E) X) u E'
+Proof
     rpt GEN_TAC
  >> EQ_TAC
  >| [ (* goal 1 (of 2) *)
@@ -808,135 +840,358 @@ val TRANS_REC_EQ = store_thm ("TRANS_REC_EQ",
       rpt STRIP_TAC \\
       PURE_ASM_REWRITE_TAC [],
       (* goal 2 (of 2) *)
-      PURE_ONCE_REWRITE_TAC [REC] ]);
+      PURE_ONCE_REWRITE_TAC [REC] ]
+QED
 
 val TRANS_REC = save_thm ("TRANS_REC", EQ_IMP_LR TRANS_REC_EQ);
 
-(******************************************************************************)
-(*                                                                            *)
-(*                     Variables and Names (Labels) in CCS                    *)
-(*                                                                            *)
-(******************************************************************************)
+(**********************************************************************)
+(*              Free and bound (recursion) variables                  *)
+(**********************************************************************)
 
 (* ('a, 'b) CCS -> 'a set (set of free variables) *)
-val FV_def = Define `
-   (FV (nil :('a, 'b) CCS)    = (EMPTY :'a set)) /\
-   (FV (prefix u p)           = FV p) /\
-   (FV (sum p q)              = (FV p) UNION (FV q)) /\
-   (FV (par p q)              = (FV p) UNION (FV q)) /\
-   (FV (restr L p)            = FV p) /\
-   (FV (relab p rf)           = FV p) /\
-   (FV (var X)                = {X}) /\
-   (FV (rec X p)              = (FV p) DIFF {X}) `;
+Definition FV_def :
+   (FV (nil :('a, 'b) CCS) = (EMPTY :'a set)) /\
+   (FV (prefix u p)        = FV p) /\
+   (FV (sum p q)           = (FV p) UNION (FV q)) /\
+   (FV (par p q)           = (FV p) UNION (FV q)) /\
+   (FV (restr L p)         = FV p) /\
+   (FV (relab p rf)        = FV p) /\
+   (FV (var X)             = {X}) /\
+   (FV (rec X p)           = (FV p) DELETE X)
+End
+
+Theorem FV_SUBSET :
+    !X E E'. FV (CCS_Subst E E' X) SUBSET (FV E) UNION (FV E')
+Proof
+    GEN_TAC >> Induct_on `E`
+ >> RW_TAC lset_ss [FV_def, CCS_Subst_def]
+ >> ASM_SET_TAC []
+QED
+
+Theorem FV_SUBSET_REC :
+    !X E. FV (CCS_Subst E (rec X E) X) SUBSET (FV E)
+Proof
+    rpt GEN_TAC
+ >> ASSUME_TAC (Q.SPECL [`X`, `E`, `rec X E`] FV_SUBSET)
+ >> ASM_SET_TAC [FV_def]
+QED
+
+(* The magical proof of TRANS_FV : (by induction on `TRANS`)
+
+        FV E' ⊆ FV E DELETE X
+   ------------------------------------
+    0.  CCS_Subst E (rec X E) X --u-> E'
+    1.  FV E' ⊆ FV (CCS_Subst E (rec X E) X)
+    2.  FV (CCS_Subst E (rec X E) X) ⊆ FV E
+    3.  FV E' ⊆ FV E
+
+  It's possible that X is a free variable in E, and then
+ `CCS_Subst E (rec X E) X` changed X into a bound variable by
+  replacing every (free) `var X` in E with `rec X (...)`,
+  that's why `FV (CCS_Subst E (rec X E) X) ⊆ FV E`.
+
+  Is X in (BV E')? Yes, possible.
+
+  Is X in (FV E')? No. Because if it's in (FV E'), it must
+  be also in FV (CCS_Subst E (rec X E) X), but this should
+  be impossible as `CCS_Subst E (rec X E) X` as turned
+  all free X into bound X. Proven by induction on X.
+ *)
+Theorem NOTIN_FV :
+    !X E E'. X NOTIN FV (CCS_Subst E (rec X E') X)
+Proof
+    GEN_TAC >> Induct_on `E`
+ >> RW_TAC lset_ss [CCS_Subst_def, FV_def]
+QED
+
+Theorem TRANS_FV :
+    !E u E'. TRANS E u E' ==> FV E' SUBSET (FV E)
+Proof
+    HO_MATCH_MP_TAC TRANS_strongind
+ >> RW_TAC lset_ss [FV_def] (* 7 subgoals *)
+ >- ASM_SET_TAC [] (* 1 *)
+ >- ASM_SET_TAC [] (* 2 *)
+ >- ASM_SET_TAC [] (* 3 *)
+ >- ASM_SET_TAC [] (* 4 *)
+ >- ASM_SET_TAC [] (* 5 *)
+ >- ASM_SET_TAC [] (* 6 *)
+ >> ASSUME_TAC (Q.SPECL [`X`, `E`] FV_SUBSET_REC)
+ >> `FV E' SUBSET FV E` by PROVE_TAC [SUBSET_TRANS]
+ >> Suff `X NOTIN (FV E')` >- ASM_SET_TAC []
+ >> CCONTR_TAC >> fs [] (* reductio ad absurdum *)
+ >> `X IN FV (CCS_Subst E (rec X E) X)` by ASM_SET_TAC []
+ >> METIS_TAC [NOTIN_FV]
+QED
+
+val lemma1 = Q.prove (
+   `!X E. X NOTIN (FV E) ==> !E'. (CCS_Subst E E' X = E)`,
+    GEN_TAC >> Induct_on `E` (* 8 subgoals *)
+ >> RW_TAC lset_ss [CCS_Subst_def, FV_def] (* one left *)
+ >> Cases_on `a = X` >- fs []
+ >> RES_TAC >> ASM_SIMP_TAC std_ss []);
+
+val lemma2 = Q.prove (
+   `!X E. (!E'. CCS_Subst E E' X = E) ==> X NOTIN (FV E)`,
+    GEN_TAC >> Induct_on `E` (* 8 subgoals *)
+ >> RW_TAC lset_ss [CCS_Subst_def, FV_def] (* 2 goals left *)
+ >- (CCONTR_TAC >> fs [] \\
+     PROVE_TAC [Q.SPEC `var a` CCS_distinct_exists])
+ >> Cases_on `X = a` >- fs []
+ >> DISJ1_TAC >> fs []);
+
+(* X is not a free variable of E if and only if E{E'/X} = E *)
+Theorem CCS_Subst_elim :
+    !X E. X NOTIN (FV E) <=> !E'. (CCS_Subst E E' X = E)
+Proof
+    METIS_TAC [lemma1, lemma2]
+QED
+
+(* if E[t/X] = E[t'/X] for all t t', X must not be free in E *)
+Theorem CCS_Subst_IMP_NO_FV :
+    !X E. (!E1 E2. CCS_Subst E E1 X = CCS_Subst E E2 X) ==> X NOTIN (FV E)
+Proof
+    Suff `!X E. X IN (FV E) ==> ?E1 E2. CCS_Subst E E1 X <> CCS_Subst E E2 X`
+ >- METIS_TAC []
+ >> GEN_TAC >> Induct_on `E` (* 8 subgoals *)
+ >> RW_TAC lset_ss [CCS_Subst_def, FV_def] (* 5 subgoals left *)
+ >- (Q.EXISTS_TAC `nil` >> METIS_TAC [CCS_distinct_exists])
+ >| [ RES_TAC >> take [`E1`, `E2`] >> DISJ1_TAC >> art [],
+      RES_TAC >> take [`E1`, `E2`] >> DISJ2_TAC >> art [],
+      RES_TAC >> take [`E1`, `E2`] >> DISJ1_TAC >> art [],
+      RES_TAC >> take [`E1`, `E2`] >> DISJ2_TAC >> art [] ]
+QED
+
+Theorem FV_PREF :
+    !X E u E'. FV (CCS_Subst E (rec X (prefix u E')) X) =
+               FV (CCS_Subst E (rec X E') X)
+Proof
+    GEN_TAC >> Induct_on `E`
+ >> RW_TAC lset_ss [CCS_Subst_def, FV_def]
+QED
+
+Theorem FV_SUM :
+    !X E E1 E2. FV (CCS_Subst E (rec X (E1 + E2)) X) =
+               (FV (CCS_Subst E (rec X E1) X)) UNION (FV (CCS_Subst E (rec X E2) X))
+Proof
+    GEN_TAC >> Induct_on `E`
+ >> RW_TAC lset_ss [CCS_Subst_def, FV_def] (* 4 subgoals *)
+ >> SET_TAC []
+QED
+
+Theorem FV_PAR :
+    !X E E1 E2. FV (CCS_Subst E (rec X (E1 || E2)) X) =
+               (FV (CCS_Subst E (rec X E1) X)) UNION (FV (CCS_Subst E (rec X E2) X))
+Proof
+    GEN_TAC >> Induct_on `E`
+ >> RW_TAC lset_ss [CCS_Subst_def, FV_def] (* 4 subgoals *)
+ >> SET_TAC []
+QED
 
 (* ('a, 'b) CCS -> 'a set (set of bound variables) *)
-val BV_def = Define `
-   (BV (nil :('a, 'b) CCS)    = (EMPTY :'a set)) /\
-   (BV (prefix u p)           = BV p) /\
-   (BV (sum p q)              = (BV p) UNION (BV q)) /\
-   (BV (par p q)              = (BV p) UNION (BV q)) /\
-   (BV (restr L p)            = BV p) /\
-   (BV (relab p rf)           = BV p) /\
-   (BV (var X)                = EMPTY) /\
-   (BV (rec X p)              = X INSERT (BV p)) `;
+Definition BV_def :
+   (BV (nil :('a, 'b) CCS) = (EMPTY :'a set)) /\
+   (BV (prefix u p)        = BV p) /\
+   (BV (sum p q)           = (BV p) UNION (BV q)) /\
+   (BV (par p q)           = (BV p) UNION (BV q)) /\
+   (BV (restr L p)         = BV p) /\
+   (BV (relab p rf)        = BV p) /\
+   (BV (var X)             = EMPTY) /\
+   (BV (rec X p)           = X INSERT (BV p))
+End
 
-val IS_PROC_def = Define `
-    IS_PROC E = (FV E = EMPTY)`;
+Theorem BV_SUBSET :
+    !X E E'. BV (CCS_Subst E E' X) SUBSET (BV E) UNION (BV E')
+Proof
+    GEN_TAC >> Induct_on `E`
+ >> RW_TAC lset_ss [BV_def, CCS_Subst_def]
+ >> ASM_SET_TAC []
+QED
 
-val ALL_PROC_def = Define `
-    ALL_PROC ES = EVERY IS_PROC ES`;
+Theorem BV_SUBSET_REC :
+    !X E. BV (CCS_Subst E (rec X E) X) SUBSET (X INSERT (BV E))
+Proof
+    rpt GEN_TAC
+ >> ASSUME_TAC (Q.SPECL [`X`, `E`, `rec X E`] BV_SUBSET)
+ >> ASM_SET_TAC [BV_def]
+QED
 
-(* The use of finite_mapTheory (to get rid of substitution orders) is
-   suggested by Konrad Slind. *)
-val CCS_Subst1_def = Define `
-   (CCS_Subst1 nil         (fm :'a |-> ('a, 'b) CCS) = nil) /\
-   (CCS_Subst1 (prefix u E) fm = prefix u (CCS_Subst1 E fm)) /\
-   (CCS_Subst1 (sum E1 E2)  fm = sum (CCS_Subst1 E1 fm)
-                                     (CCS_Subst1 E2 fm)) /\
-   (CCS_Subst1 (par E1 E2)  fm = par (CCS_Subst1 E1 fm)
-                                     (CCS_Subst1 E2 fm)) /\
-   (CCS_Subst1 (restr L E)  fm = restr L (CCS_Subst1 E fm)) /\
-   (CCS_Subst1 (relab E rf) fm = relab   (CCS_Subst1 E fm) rf) /\
-   (CCS_Subst1 (var Y)      fm = if (Y IN FDOM fm) then (FAPPLY fm Y)
-                                 else (var Y)) /\
-   (CCS_Subst1 (rec Y E)    fm = if (Y IN FDOM fm) then (rec Y E)
-                                 else (rec Y (CCS_Subst1 E fm)))`;
+Theorem TRANS_BV :
+    !E u E'. TRANS E u E' ==> BV E' SUBSET BV E
+Proof
+    HO_MATCH_MP_TAC TRANS_ind
+ >> RW_TAC lset_ss [BV_def] (* 7 subgoals *)
+ >- ASM_SET_TAC [] (* 1 *)
+ >- ASM_SET_TAC [] (* 2 *)
+ >- ASM_SET_TAC [] (* 3 *)
+ >- ASM_SET_TAC [] (* 4 *)
+ >- ASM_SET_TAC [] (* 5 *)
+ >- ASM_SET_TAC [] (* 6 *)
+ >> MATCH_MP_TAC SUBSET_TRANS
+ >> Q.EXISTS_TAC `BV (CCS_Subst E (rec X E) X)`
+ >> fs [BV_SUBSET_REC]
+QED
 
-(* :('a, 'b) CCS list -> ('a |-> ('a, 'b) CCS) -> ('a, 'b) CCS list *)
-val CCS_Subst2_def = Define `
-    CCS_Subst2 ES fm = MAP (\e. CCS_Subst1 e fm) ES`;
+Theorem TRANS_FV_old :
+    !E u E'. TRANS E u E' ==> FV E' SUBSET (FV E UNION BV E)
+Proof
+    HO_MATCH_MP_TAC TRANS_strongind
+ >> RW_TAC lset_ss [BV_def, FV_def] (* 9 subgoals *)
+ >- ASM_SET_TAC [] (* 1 *)
+ >- ASM_SET_TAC [] (* 2 *)
+ >- ASM_SET_TAC [] (* 3 *)
+ >- ASM_SET_TAC [] (* 4 *)
+ >- ASM_SET_TAC [] (* 5 *)
+ >- ASM_SET_TAC [] (* 6 *)
+ >- ASM_SET_TAC [] (* 7 *)
+ >- ASM_SET_TAC [] (* 8 *)
+ >> ASSUME_TAC (Q.SPECL [`X`, `E`] FV_SUBSET_REC)
+ >> ASSUME_TAC (Q.SPECL [`X`, `E`] BV_SUBSET_REC)
+ >> Q.ABBREV_TAC `A = FV (CCS_Subst E (rec X E) X)`
+ >> Q.ABBREV_TAC `B = BV (CCS_Subst E (rec X E) X)`
+ >> MATCH_MP_TAC SUBSET_TRANS
+ >> Q.EXISTS_TAC `A UNION B` >> art []
+ >> ASM_SET_TAC []
+QED
 
-val DELETE_ELEMENT_def = Define `
-   (DELETE_ELEMENT e [] = []) /\
-   (DELETE_ELEMENT e (x :: l) =
-    if (e = x) then DELETE_ELEMENT e l else x :: DELETE_ELEMENT e l)`;
+Theorem BV_REC :
+    !X E. X IN BV (rec X E)
+Proof
+    RW_TAC std_ss [BV_def, IN_INSERT]
+QED
 
-val NOT_IN_DELETE_ELEMENT = store_thm (
-   "NOT_IN_DELETE_ELEMENT",
-  ``!e L. ~MEM e (DELETE_ELEMENT e L)``,
+Theorem BV_SUBSET_rules :
+    !X E E'. (BV E) SUBSET (BV (rec X E)) /\
+             (BV E) SUBSET (BV (sum E E')) /\ (BV E') SUBSET (BV (sum E E')) /\
+             (BV E) SUBSET (BV (par E E')) /\ (BV E') SUBSET (BV (par E E'))
+Proof
+    rpt GEN_TAC >> SET_TAC [BV_def]
+QED
+
+Definition IS_PROC_def :
+    IS_PROC P <=> (FV P = EMPTY)
+End
+
+Definition ALL_PROC_def :
+    ALL_PROC Ps <=> EVERY IS_PROC Ps
+End
+
+Theorem IS_PROC_EL :
+    !Ps n. ALL_PROC Ps /\ n < LENGTH Ps ==> IS_PROC (EL n Ps)
+Proof
+    RW_TAC list_ss [ALL_PROC_def, EVERY_MEM, MEM_EL]
+ >> FIRST_X_ASSUM MATCH_MP_TAC
+ >> Q.EXISTS_TAC `n` >> art []
+QED
+
+Theorem IS_PROC_prefix :
+    !P u. IS_PROC (prefix u P) <=> IS_PROC P
+Proof
+    RW_TAC std_ss [IS_PROC_def, FV_def]
+QED
+
+Theorem IS_PROC_sum :
+    !P Q. IS_PROC (sum P Q) <=> IS_PROC P /\ IS_PROC Q
+Proof
+    RW_TAC lset_ss [IS_PROC_def, FV_def]
+QED
+
+Theorem IS_PROC_par :
+    !P Q. IS_PROC (par P Q) <=> IS_PROC P /\ IS_PROC Q
+Proof
+    RW_TAC lset_ss [IS_PROC_def, FV_def]
+QED
+
+Theorem IS_PROC_restr :
+    !P L. IS_PROC (restr L P) <=> IS_PROC P
+Proof
+    RW_TAC lset_ss [IS_PROC_def, FV_def]
+QED
+
+Theorem IS_PROC_relab :
+    !P rf. IS_PROC (relab P rf) <=> IS_PROC P
+Proof
+    RW_TAC lset_ss [IS_PROC_def, FV_def]
+QED
+
+Theorem TRANS_PROC :
+    !E u E'. TRANS E u E' /\ IS_PROC E ==> IS_PROC E'
+Proof
+    RW_TAC std_ss [IS_PROC_def]
+ >> `FV E' SUBSET FV E` by PROVE_TAC [TRANS_FV]
+ >> rfs []
+QED
+
+(**********************************************************************)
+(*                Free and bound names (sorts) ('b)                   *)
+(**********************************************************************)
+
+(* To be moved to rich_listTheory *)
+Definition DELETE_ELEMENT :
+    (DELETE_ELEMENT e [] = []) /\
+    (DELETE_ELEMENT e (x :: l) = if (e = x) then DELETE_ELEMENT e l
+                                 else x :: DELETE_ELEMENT e l)
+End
+
+Theorem NOT_IN_DELETE_ELEMENT :
+    !e L. ~MEM e (DELETE_ELEMENT e L)
+Proof
     GEN_TAC >> Induct_on `L`
- >- REWRITE_TAC [DELETE_ELEMENT_def, MEM]
- >> GEN_TAC >> REWRITE_TAC [DELETE_ELEMENT_def]
- >> Cases_on `e = h` >> fs []);
+ >- REWRITE_TAC [DELETE_ELEMENT, MEM]
+ >> GEN_TAC >> REWRITE_TAC [DELETE_ELEMENT]
+ >> Cases_on `e = h` >> fs []
+QED
 
-val DELETE_ELEMENT_FILTER = store_thm (
-   "DELETE_ELEMENT_FILTER",
-  ``!e L. DELETE_ELEMENT e L = FILTER ((<>) e) L``,
+Theorem DELETE_ELEMENT_FILTER :
+    !e L. DELETE_ELEMENT e L = FILTER ((<>) e) L
+Proof
     GEN_TAC >> Induct_on `L`
- >- REWRITE_TAC [DELETE_ELEMENT_def, FILTER]
- >> GEN_TAC >> REWRITE_TAC [DELETE_ELEMENT_def, FILTER]
- >> Cases_on `e = h` >> fs []);
+ >- REWRITE_TAC [DELETE_ELEMENT, FILTER]
+ >> GEN_TAC >> REWRITE_TAC [DELETE_ELEMENT, FILTER]
+ >> Cases_on `e = h` >> fs []
+QED
 
-val LENGTH_DELETE_ELEMENT_LEQ = store_thm (
-   "LENGTH_DELETE_ELEMENT_LEQ",
-  ``!e L. LENGTH (DELETE_ELEMENT e L) <= LENGTH L``,
+Theorem LENGTH_DELETE_ELEMENT_LEQ :
+    !e L. LENGTH (DELETE_ELEMENT e L) <= LENGTH L
+Proof
     rpt GEN_TAC
  >> REWRITE_TAC [DELETE_ELEMENT_FILTER]
  >> MP_TAC (Q.SPECL [`\y. e <> y`, `\y. T`] LENGTH_FILTER_LEQ_MONO)
- >> BETA_TAC >> simp []);
+ >> BETA_TAC >> simp []
+QED
 
-val LENGTH_DELETE_ELEMENT_LE = store_thm (
-   "LENGTH_DELETE_ELEMENT_LE",
-  ``!e L. MEM e L ==> LENGTH (DELETE_ELEMENT e L) < LENGTH L``,
+Theorem LENGTH_DELETE_ELEMENT_LE :
+    !e L. MEM e L ==> LENGTH (DELETE_ELEMENT e L) < LENGTH L
+Proof
     rpt GEN_TAC >> Induct_on `L`
  >- REWRITE_TAC [MEM]
- >> GEN_TAC >> REWRITE_TAC [MEM, DELETE_ELEMENT_def]
+ >> GEN_TAC >> REWRITE_TAC [MEM, DELETE_ELEMENT]
  >> Cases_on `e = h` >> fs []
  >> MP_TAC (Q.SPECL [`h`, `L`] LENGTH_DELETE_ELEMENT_LEQ)
- >> KILL_TAC >> RW_TAC arith_ss []);
+ >> KILL_TAC >> RW_TAC arith_ss []
+QED
 
-val EVERY_DELETE_ELEMENT = store_thm (
-   "EVERY_DELETE_ELEMENT",
-  ``!e L P. P e /\ EVERY P (DELETE_ELEMENT e L) ==> EVERY P L``,
+Theorem EVERY_DELETE_ELEMENT :
+    !e L P. P e /\ EVERY P (DELETE_ELEMENT e L) ==> EVERY P L
+Proof
     GEN_TAC >> Induct_on `L`
- >- RW_TAC std_ss [DELETE_ELEMENT_def]
- >> rpt GEN_TAC >> REWRITE_TAC [DELETE_ELEMENT_def]
- >> Cases_on `e = h` >> fs []);
+ >- RW_TAC std_ss [DELETE_ELEMENT]
+ >> rpt GEN_TAC >> REWRITE_TAC [DELETE_ELEMENT]
+ >> Cases_on `e = h` >> fs []
+QED
 
-val DELETE_ELEMENT_APPEND = store_thm (
-   "DELETE_ELEMENT_APPEND",
-  ``!a L L'. DELETE_ELEMENT a (L ++ L') = DELETE_ELEMENT a L ++ DELETE_ELEMENT a L'``,
+Theorem DELETE_ELEMENT_APPEND :
+    !a L L'. DELETE_ELEMENT a (L ++ L') =
+             DELETE_ELEMENT a L ++ DELETE_ELEMENT a L'
+Proof
     REWRITE_TAC [DELETE_ELEMENT_FILTER]
- >> REWRITE_TAC [GSYM FILTER_APPEND_DISTRIB]);
+ >> REWRITE_TAC [GSYM FILTER_APPEND_DISTRIB]
+QED
 
-(* not used so far, learnt from Robert Beers *)
-val ALL_IDENTICAL_def = Define `
-    ALL_IDENTICAL t = ?x. !y. MEM y t ==> (y = x)`;
-
-(*
-You might define the sublist relation: (from Michael Norrish)
-Sublist [] l = T
-  Sublist _ [] = F
-  Sublist (h1::t1) (h2::t2) = if h1 = h2 then Sublist t1 t2 else Sublist (h1::t1) t2
-
-And show that
-
-  Sublist (DELETE_ELEMENT e l) l
-*)
-
-(* (size :(α, β) CCS -> num) *)
-val size_def = Define `
-    size (p :('a, 'b) CCS) = ^CCS_size_tm (\x. 0) (\x. 0) p`;
+(* Learnt from Robert Beers (not used so far) *)
+Definition ALL_IDENTICAL :
+    ALL_IDENTICAL t = ?x. !y. MEM y t ==> (y = x)
+End
 
 (* (FN :('a, 'b) CCS -> 'a list -> 'b Label set) *)
 val FN_definition = `
@@ -946,7 +1201,7 @@ val FN_definition = `
    (FN (sum p q) J            = (FN p J) UNION (FN q J)) /\
    (FN (par p q) J            = (FN p J) UNION (FN q J)) /\
    (FN (restr L p) J          = (FN p J) DIFF (L UNION (IMAGE COMPL_LAB L))) /\
-   (FN (relab p rf) J         = IMAGE (REP_Relabeling rf) (FN p J)) /\
+   (FN (relab p rf) J         = IMAGE (REP_Relabeling rf) (FN p J)) /\ (* here *)
    (FN (var X) J              = EMPTY) /\
    (FN (rec X p) J            = if (MEM X J) then
                                     FN (CCS_Subst p (rec X p) X) (DELETE_ELEMENT X J)
@@ -958,11 +1213,11 @@ val BN_definition = `
    (BN (prefix u p) J         = BN p J) /\
    (BN (sum p q) J            = (BN p J) UNION (BN q J)) /\
    (BN (par p q) J            = (BN p J) UNION (BN q J)) /\
-   (BN (restr L p) J          = (BN p J) UNION L) /\    (* here! *)
+   (BN (restr L p) J          = (BN p J) UNION L) /\ (* here *)
    (BN (relab p rf) J         = BN p J) /\
    (BN (var X) J              = EMPTY) /\
    (BN (rec X p) J            = if (MEM X J) then
-                                    FN (CCS_Subst p (rec X p) X) (DELETE_ELEMENT X J)
+                                    BN (CCS_Subst p (rec X p) X) (DELETE_ELEMENT X J)
                                 else EMPTY)`;
 
 (* This is how we get the correct tactics (FN_tac):
@@ -970,23 +1225,26 @@ val BN_definition = `
  - Defn.tgoal FN_defn;
  *)
 local
-    val tactic = (* the use of `($< LEX $<)` is learnt from Ramana Kumar *)
-        WF_REL_TAC `inv_image ($< LEX $<) (\x. (LENGTH (SND x), size (FST x)))`
-     >> rpt STRIP_TAC >- ( IMP_RES_TAC LENGTH_DELETE_ELEMENT_LE >> art [] )
-     >> REWRITE_TAC [size_def, CCS_size_def]
-     >> simp [];
+  val tactic = (* the use of `($< LEX $<)` is learnt from Ramana Kumar *)
+      WF_REL_TAC `inv_image ($< LEX $<)
+                            (\x. (LENGTH (SND x), ^CCS_size_tm (\x. 0) (\x. 0) (FST x)))`
+   >> rpt STRIP_TAC >- (IMP_RES_TAC LENGTH_DELETE_ELEMENT_LE >> art [])
+   >> REWRITE_TAC [CCS_size_def]
+   >> simp [];
 in
-    val FN_def = TotalDefn.tDefine "FN" FN_definition tactic;
-    val BN_def = TotalDefn.tDefine "BN" BN_definition tactic;
+  val FN_def = TotalDefn.tDefine "FN" FN_definition tactic;
+  val BN_def = TotalDefn.tDefine "BN" BN_definition tactic;
 end;
 
-(* (free_names :('a, 'b) CCS -> 'b Label set) collects all visible labels in the prefix *)
-val free_names_def = Define ` (* also called "sorts" by Robin Milner *)
-    free_names p = FN p (SET_TO_LIST (BV p))`;
+(* (free_names :('a, 'b) CCS -> 'b Label set) collects all visible
+   labels (also called "sorts") as the prefix, w.r.t relabeling operators. *)
+val free_names_def = Define
+   `free_names p = FN p (SET_TO_LIST (BV p))`;
 
-(* (bound_names :('a, 'b) CCS -> 'b Label set) collects all visible labels in the restr *)
-val bound_names_def = Define `
-    bound_names p = BN p (SET_TO_LIST (BV p))`;
+(* (bound_names :('a, 'b) CCS -> 'b Label set) collects all visible
+   labels by the restriction operator. *)
+val bound_names_def = Define
+   `bound_names p = BN p (SET_TO_LIST (BV p))`;
 
 val FN_UNIV1 = store_thm ("FN_UNIV1",
   ``!p. free_names p <> (UNIV :'b Label set) ==> ?a. a NOTIN free_names p``,
@@ -999,5 +1257,3 @@ val FN_UNIV2 = store_thm ("FN_UNIV2",
 
 val _ = export_theory ();
 val _ = html_theory "CCS";
-
-(* last updated: Oct 24, 2017 *)
